BourbakiLean2/Function/Rel.lean
@@ -1,0 +1,68 @@
+import BourbakiLean2.Function.Basic
+
+namespace Relation
+variable {α β γ δ : Type*} {f : α → β} {g : γ → α}
+variable {r r' : Relation α β}
+
+def proj1 (r : Relation α β) : ↑ r → ↑ r.domain
+| ⟨⟨a,_⟩,h⟩ => ⟨a, mem_domain_of h⟩
+
+def proj2 (r : Relation α β) : ↑ r → ↑ r.range
+| ⟨⟨_,b⟩,h⟩ => ⟨b, mem_range_of h⟩
+
+@[simp] theorem proj1_val {a : _} : proj1 r a = ((↑ a) : α × β).1 := by
+  dsimp only [proj1]
+
+@[simp] theorem proj2_val {a : _} : proj2 r a = ((↑ a) : α × β).2 := by
+  dsimp only [proj2]
+
+@[simp] theorem proj1_val' {a b h : _} : proj1 r ⟨⟨a,b⟩,h⟩ = a := by
+  dsimp only [proj1_val]
+
+@[simp] theorem proj2_val' {a b h : _} : proj2 r ⟨⟨a,b⟩,h⟩ = b := by
+  dsimp only [proj2_val]
+
+theorem proj1_surj : Function.Surjective (proj1 r) := by
+  simp only [Function.surj_iff, Subtype.exists, Prod.exists, Subtype.forall, mem_domain_iff,
+    forall_exists_index]
+  intro a b h
+  exists a
+  exists b
+  exists h
+
+theorem proj2_surj : Function.Surjective (proj2 r) := by
+  simp only [Function.surj_iff, Subtype.exists, Prod.exists, Subtype.forall, mem_range_iff,
+    forall_exists_index]
+  intro a b h
+  exists b
+  exists a
+  exists h
+
+
+def proj1_inj_domain_iff_functional : (Function.Injective (proj1 r) ∧ r.domain = Set.univ) ↔ r.Functional := by
+  constructor
+  · rintro ⟨h,h'⟩ a
+    rw[Set.ext_iff] at h'
+    specialize h' a
+    simp only [mem_domain_iff, Set.mem_univ, iff_true] at h'
+    obtain ⟨b, h''⟩ := h'
+    exists b
+    simp only [h'', true_and]
+    intro b' h'''
+    specialize h ⟨(a,b),h''⟩ ⟨(a,b'),h'''⟩
+    simp only [Subtype.mk.injEq, Prod.mk.injEq, true_and] at h
+    apply Eq.symm ∘ h
+    simp only [Subtype.eq_iff, proj1_val]
+  · intro h
+    constructor
+    · rintro ⟨⟨a,b⟩, h'⟩ ⟨⟨a',b'⟩,h''⟩ h'''
+      simp only [Subtype.eq_iff, proj1_val] at *
+      simp only [h''', Prod.mk.injEq, true_and] at *
+      specialize h a'
+      obtain ⟨_,⟨_,h⟩⟩ := h
+      have hb := h b h'
+      have hb' := h b' h''
+      rw[hb, hb']
+    · exact domain_functional h
+
+end Relation
